Augmented semantics + logics to support function definitions.

theories/Hoare.v
@@ -11,94 +11,77 @@ Require Import Maps Imp HoareCommon.
 
 Section Hoare.
 
-Context {env : Env}.
+  Reserved Notation "Sigma |- {{ P }}  c  {{ Q }}"
+           (at level 90, c at next level).
 
-Definition hoare_triple
-           (P : Assertion) (c : com) (Q : Assertion) : Prop :=
-  forall st st',
-     st =[ c ]=> st'  ->
-     P st  ->
-     Q st'.
-
-Notation "{{ P }}  c  {{ Q }}" :=
-  (hoare_triple P c Q) (at level 90, c at next level)
-  : hoare_spec_scope.
-
-Definition wp (c:com) (Q:Assertion) : Assertion :=
-  fun s => forall s', s =[ c ]=> s' -> Q s'.
-
-Lemma wp_is_precondition: forall c Q,
-  {{wp c Q}} c {{Q}}.
-Proof.
-  firstorder.
-Qed.
-
-Lemma wp_is_weakest: forall c Q P',
-   {{P'}} c {{Q}} -> forall st, P' st -> wp c Q st.
-Proof.
-  firstorder.
-Qed.
-
-Reserved Notation "|- {{ P }}  c  {{ Q }}"
-         (at level 90, c at next level).
-
-Inductive hoare_proof : Assertion -> com -> Assertion -> Type :=
+  Inductive hoare_proof (Sigma : total_map funSpec) : Assertion -> com -> Assertion -> Prop :=
   | H_Skip : forall P,
-      |- {{P}} SKIP {{P}}
+      Sigma |- {{P}} SKIP {{P}}
   | H_Asgn : forall Q V a,
-      |- {{Q[V |-> a]}} V ::= a {{Q}}
-  | H_Spec : forall Q y f xs,
-      |- {{fun st =>
-            (funsig f).(pre) (aseval st xs) ->
-            forall v, (funsig f).(post) v (aseval st xs) ->
-                 Q[y |-> v] st}} y :::= f $ xs {{Q}}
+      Sigma |- {{Q[V |-> a]}} V ::= a {{Q}}
   | H_Seq  : forall P c Q d R,
-      |- {{P}} c {{Q}} -> |- {{Q}} d {{R}} ->
-      |- {{P}} c;;d {{R}}
+      Sigma|- {{P}} c {{Q}} ->
+      Sigma |- {{Q}} d {{R}} ->
+      Sigma |- {{P}} c;;d {{R}}
   | H_If : forall P Q b c1 c2,
-      |- {{fun st => P st /\ bassn b st}} c1 {{Q}} ->
-      |- {{fun st => P st /\ ~(bassn b st)}} c2 {{Q}} ->
-      |- {{P}} TEST b THEN c1 ELSE c2 FI {{Q}}
+      Sigma |- {{fun st => P st /\ bassn b st}} c1 {{Q}} ->
+      Sigma |- {{fun st => P st /\ ~(bassn b st)}} c2 {{Q}} ->
+      Sigma |- {{P}} TEST b THEN c1 ELSE c2 FI {{Q}}
   | H_While : forall P b c,
-      |- {{fun st => P st /\ bassn b st}} c {{P}} ->
-      |- {{P}} WHILE b DO c END {{fun st => P st /\ ~ (bassn b st)}}
+      Sigma |- {{fun st => P st /\ bassn b st}} c {{P}} ->
+      Sigma |- {{P}} WHILE b DO c END {{fun st => P st /\ ~ (bassn b st)}}
   | H_Consequence  : forall (P Q P' Q' : Assertion) c,
-      |- {{P'}} c {{Q'}} ->
+      Sigma |- {{P'}} c {{Q'}} ->
       (forall st, P st -> P' st) ->
       (forall st, Q' st -> Q st) ->
-      |- {{P}} c {{Q}}
+      Sigma |- {{P}} c {{Q}}
 
-where "|- {{ P }}  c  {{ Q }}" := (hoare_proof P c Q) : hoare_spec_scope.
+  | H_Call : forall Q y f xs,
+      Sigma |- {{fun st =>
+            (Sigma f).(pre) (aseval st xs) ->
+            forall v, (Sigma f).(post) v (aseval st xs) ->
+                 Q[y |-> v] st}} y :::= f $ xs {{Q}}
 
 
-Hint Resolve bassn_eval_true bassn_eval_false : hoare.
-Hint Resolve wp_is_precondition wp_is_weakest : hoare.
-Hint Constructors hoare_proof : hoare.
-Hint Unfold hoare_triple wp.
-Hint Constructors ceval.
+where "Sigma |- {{ P }}  c  {{ Q }}" := (hoare_proof Sigma P c Q) : hoare_spec_scope.
 
-Lemma hoare_while : forall P b c,
-    {{fun st => P st /\ bassn b st}} c {{P}} ->
-    {{P}} WHILE b DO c END {{fun st => P st /\ ~ (bassn b st)}}.
-Proof.
-  unfold hoare_triple.
-  intros ? ? ? ? ? ? HE ?. remember (WHILE b DO c END)%imp eqn:Heq.
-  induction HE; try inversion Heq; subst.
-  - firstorder with hoare.
-  - eauto.
-Qed.
+  Definition hoare_triple
+             {env : Env}
+             (P : Assertion) (c : com) (Q : Assertion) : Prop :=
+    forall st st',
+      st =[ c ]=> st'  ->
+      P st  ->
+      Q st'.
 
-Theorem hoare_proof_sound : forall P c Q,
-    |- {{P}} c {{Q}} -> {{P}} c {{Q}}.
-Proof.
-  unfold hoare_triple.
+  Notation "{{ P }}  c  {{ Q }}" :=
+    (hoare_triple P c Q) (at level 90, c at next level)
+    : hoare_spec_scope.
+
+  Hint Resolve bassn_eval_true bassn_eval_false : hoare.
+  Hint Constructors hoare_proof : hoare.
+  Hint Unfold hoare_triple.
+  Hint Constructors ceval.
+
+  Lemma hoare_while {env : Env} : forall P b c,
+      {{fun st => P st /\ bassn b st}} c {{P}} ->
+      {{P}} WHILE b DO c END {{fun st => P st /\ ~ (bassn b st)}}.
+  Proof.
+    unfold hoare_triple.
+    intros ? ? ? ? ? ? HE ?. remember (WHILE b DO c END)%imp eqn:Heq.
+    induction HE; try inversion Heq; subst.
+    - firstorder with hoare.
+    - eauto.
+  Qed.
+
+  Theorem hoare_proof_sound Sigma : forall P c Q,
+      Sigma |- {{P}} c {{Q}} ->
+      @hoare_triple {| funSpecs := Sigma; funDefs := empty |} P c Q.
+  Proof.
   intros ? ? ? pf. induction pf; intros st st' HE HP.
   - (* SKIP *)
     inversion HE; subst. eauto.
   - (* ::= *)
     inversion HE; subst. eauto.
-  - (* :::= *)
-    inversion HE; subst. firstorder.
   - (* ;; *)
     inversion HE; subst. eauto.
   - (* TEST *)
@@ -108,34 +91,80 @@ Proof.
     eapply hoare_while; eauto.
   - (* Conseq *)
     eauto.
-Qed.
-
-Theorem hoare_proof_complete: forall P c Q,
-    {{P}} c {{Q}} -> |- {{P}} c {{Q}}.
-Proof.
-  unfold hoare_triple.
-  intros P c. revert dependent P.
-  induction c; intros P Q HT.
-  - (* SKIP *)
-    eapply H_Consequence; eauto with hoare.
-  - (* ::= *)
-    eapply H_Consequence; eauto with hoare.
-    intros; eapply HT; eauto.
   - (* :::= *)
-    eapply H_Consequence; eauto with hoare.
-    simpl. intros. eapply HT; eauto.
-  - (* ;; *)
-    apply H_Seq with (wp c2 Q); firstorder eauto.
-  - (* IFB *)
-    apply H_If.
-    + firstorder eauto.
-    + apply IHc2. firstorder with hoare.
-  - (* WHILE *)
-    eapply H_Consequence with (P':=wp (WHILE b DO c END) Q).
-    + constructor. firstorder eauto.
-    + eauto.
-    + firstorder with hoare.
-Qed.
+    inversion HE; subst; try firstorder.
+    simpl in H4; rewrite apply_empty in H4; discriminate.
+  Qed.
+
+  Definition wp {env : Env} (c:com) (Q:Assertion) : Assertion :=
+    fun s => forall s', s =[ c ]=> s' -> Q s'.
+
+  Lemma wp_is_precondition {env : Env}: forall c Q,
+      {{wp c Q}} c {{Q}}.
+  Proof.
+    firstorder.
+  Qed.
+
+  Lemma wp_is_weakest {env : Env} : forall c Q P',
+      {{P'}} c {{Q}} -> forall st, P' st -> wp c Q st.
+  Proof.
+    firstorder.
+  Qed.
+
+  Hint Resolve wp_is_precondition wp_is_weakest : hoare.
+  Hint Unfold wp.
+
+  Theorem hoare_proof_complete Sigma : forall P c Q,
+      @hoare_triple {| funSpecs := Sigma; funDefs := empty |} P c Q->
+      Sigma |- {{P}} c {{Q}}.
+  Proof.
+    unfold hoare_triple.
+    intros P c. revert dependent P.
+    induction c; intros P Q HT.
+    - (* SKIP *)
+      eapply H_Consequence; eauto with hoare.
+    - (* ::= *)
+      eapply H_Consequence; eauto with hoare.
+      intros; eapply HT; eauto.
+    - (* :::= *)
+      eapply H_Consequence; eauto with hoare.
+      simpl. intros. eapply HT; eauto.
+    - (* ;; *)
+      apply H_Seq with (@wp {| funSpecs := Sigma; funDefs := empty |} c2 Q); firstorder eauto.
+    - (* IFB *)
+      apply H_If.
+      + firstorder eauto.
+      + apply IHc2. firstorder with hoare.
+    - (* WHILE *)
+      eapply H_Consequence with (P':= @wp {| funSpecs := Sigma; funDefs := empty |} (WHILE b DO c END) Q).
+      + constructor. firstorder eauto.
+      + eauto.
+      + firstorder with hoare.
+  Qed.
+
+  Theorem hoare_proof_link {Sigma : Env}
+    : forall (P Q : Assertion) c,
+      valid_Env Sigma ->
+      (forall st, P st -> @Safe {| funSpecs := @funSpecs Sigma; funDefs := empty |} c st) ->
+      funSpecs |- {{P}} c {{Q}} ->
+      @hoare_triple Sigma P c Q.
+  Proof.
+    intros.
+    pose proof (hoare_proof_sound _ _ _ _ H0);
+      eauto using valid_Env_refine, hoare_proof_sound.
+  Qed.
+
+  (* This one is going to require more care...*)
+  Theorem hoare_valid_Env
+    : forall {Sigma : Env},
+      (forall f fd,
+          funDefs f = Some fd ->
+          funSpecs |- {{ fun st => pre (funSpecs f) (List.map st (funArgs fd)) }}
+                        funBody fd
+                      {{ fun st => post (funSpecs f) (aeval st (funRet fd)) (List.map st (funArgs fd)) }}) ->
+      valid_Env Sigma.
+  Proof.
+  Abort.
 
 End Hoare.
 
@@ -143,6 +172,6 @@ Notation "{{ P }}  c  {{ Q }}" :=
   (hoare_triple P c Q) (at level 90, c at next level)
   : hoare_spec_scope.
 
-Notation "|- {{ P }}  c  {{ Q }}" :=
-  (hoare_proof P c Q) (at level 90, c at next level)
+Notation "Sigma |- {{ P }}  c  {{ Q }}" :=
+  (hoare_proof Sigma P c Q) (at level 90, c at next level)
   : hoare_spec_scope.
