theories/RHLE.v
@@ -3,7 +3,17 @@ Require Import
         Coq.micromega.Psatz
         Coq.Program.Tactics.
 
-Require Import Maps Imp HoareCommon Hoare EHoare.
+Require Import Maps Imp.
+
+Ltac inv_ceval :=
+  let t H := (inversion H; subst; clear H) in
+  match goal with
+  | H : _ =[ SKIP ]=> _
+                      |- _ => t H
+  | H : _ =[ _;;_ ]=> _ |- _ => t H
+  end.
+
+Require Import HoareCommon Hoare EHoare.
 
 Definition Assertion2 := state -> state -> Prop.
 
@@ -12,94 +22,87 @@ Definition assert2_implies (P Q : Assertion2) : Prop :=
 
 Section RHLE.
 
-Context {env : Env}.
+  Definition rhle_triple {env : Env}
+             (P : Assertion2) (c1 : com) (c2 : com) (Q : Assertion2) : Prop :=
+    forall st1 st2 st1',
+      st1 =[ c1 ]=> st1'  ->
+                    P st1 st2 ->
+                    exists st2' (exe : st2 =[ c2 ]=> st2'), Q st1' st2'.
 
-Definition rhle_triple
-           (P : Assertion2) (c1 : com) (c2 : com) (Q : Assertion2) : Prop :=
-  forall st1 st2 st1',
-     st1 =[ c1 ]=> st1'  ->
-     P st1 st2 ->
-     exists st2' (exe : st2 =[ c2 ]=> st2'), Q st1' st2'.
+  Notation "{{ P }}  c1 ~# c2  {[ Q ]}" :=
+    (rhle_triple P c1 c2 Q) (at level 90, c1 at next level, c2 at next level)
+    : hoare_spec_scope.
 
-Notation "{{ P }}  c1 ~# c2  {[ Q ]}" :=
-  (rhle_triple P c1 c2 Q) (at level 90, c1 at next level, c2 at next level)
-  : hoare_spec_scope.
+  Reserved Notation "Sigma |- {{ P }}  c1 ~# c2  {[ Q ]}"
+           (at level 90, c1 at next level, c2 at next level).
 
-Reserved Notation "|- {{ P }}  c1 ~# c2  {[ Q ]}"
-         (at level 90, c1 at next level, c2 at next level).
+  Inductive rhle_proof Sigma : Assertion2 -> com -> com -> Assertion2 -> Prop :=
+  | RHE_Skip : forall P,
+      Sigma |- {{P}} SKIP ~# SKIP {[P]}
+  | RHE_SkipIntroL : forall P Q c1 c2,
+      Sigma |- {{P}} c1;;SKIP ~# c2 {[Q]} ->
+      Sigma |- {{P}} c1 ~# c2 {[Q]}
+  | RHE_SkipIntroR : forall P Q c1 c2,
+      Sigma |- {{P}} c1 ~# c2;;SKIP {[Q]} ->
+      Sigma |- {{P}} c1 ~# c2 {[Q]}
+  | RHE_StepL : forall P Q R c1 c2 c3,
+      (forall st2, Sigma |- {{fun st => P st st2}} c1 {{fun st => Q st st2}}) ->
+      Sigma |- {{Q}} c2 ~# c3 {[R]} ->
+      Sigma |- {{P}} c1;;c2 ~# c3 {[R]}
+  | RHE_StepR : forall P Q R c1 c2 c3,
+      (forall st1, Sigma |- {[fun st => P st1 st]} c2 {[fun st => Q st1 st]}#) ->
+      Sigma |- {{Q}} c1 ~# c3 {[R]} ->
+      Sigma |- {{P}} c1 ~# c2;;c3 {[R]}
 
-Inductive rhle_proof : Assertion2 -> com -> com -> Assertion2 -> Prop :=
-| RHE_Skip : forall P,
-    |- {{P}} SKIP ~# SKIP {[P]}
-| RHE_SkipIntroL : forall P Q c1 c2,
-    |- {{P}} c1;;SKIP ~# c2 {[Q]} ->
-    |- {{P}} c1 ~# c2 {[Q]}
-| RHE_SkipIntroR : forall P Q c1 c2,
-    |- {{P}} c1 ~# c2;;SKIP {[Q]} ->
-    |- {{P}} c1 ~# c2 {[Q]}
-| RHE_StepL : forall P Q R c1 c2 c3,
-    (forall st2, |- {{fun st => P st st2}} c1 {{fun st => Q st st2}}) ->
-    |- {{Q}} c2 ~# c3 {[R]} ->
-    |- {{P}} c1;;c2 ~# c3 {[R]}
-| RHE_StepR : forall P Q R c1 c2 c3,
-    (forall st1, |- {[fun st => P st1 st]} c2 {[fun st => Q st1 st]}#) ->
-    |- {{Q}} c1 ~# c3 {[R]} ->
-    |- {{P}} c1 ~# c2;;c3 {[R]}
+  where "Sigma |- {{ P }}  c1 ~# c2  {[ Q ]}" := (rhle_proof Sigma P c1 c2 Q) : hoare_spec_scope.
 
-where "|- {{ P }}  c1 ~# c2  {[ Q ]}" := (rhle_proof P c1 c2 Q) : hoare_spec_scope.
+  Hint Resolve bassn_eval_true bassn_eval_false : hoare.
+  Hint Constructors rhle_proof : hoare.
+  Hint Unfold rhle_triple hoare_triple ehoare_triple.
+  Hint Constructors ceval.
 
-Hint Resolve bassn_eval_true bassn_eval_false : hoare.
-Hint Constructors rhle_proof : hoare.
-Hint Unfold rhle_triple hoare_triple ehoare_triple.
-Hint Constructors ceval.
+  Ltac apply_sound :=
+    match goal with
+    | H : context[_ |- {{_}} _ {{_}}] |- _ =>
+      eapply hoare_proof_sound in H
+    | H : context[_ |- {[_]} _ {[_]}#] |- _ =>
+      eapply ehoare_proof_sound in H
+    end.
 
-Ltac inv_ceval :=
-  let t H := (inversion H; subst; clear H) in
-  match goal with
-  | H : _ =[ SKIP ]=> _ |- _ => t H
-  | H : _ =[ _;;_ ]=> _ |- _ => t H
-  end.
+  Theorem rhle_proof_sound Sigma : forall P c1 c2 Q,
+      Sigma |- {{P}} c1 ~# c2 {[Q]} ->
+      @rhle_triple {| funSpecs := Sigma; funDefs := empty |} P c1 c2 Q.
+  Proof.
+    intros ? ? ? ? pf.
+    unfold rhle_triple.
+    induction pf; intros st1 st2 st1' exe HP.
+    - inv_ceval. eauto.
+    - firstorder eauto.
+    - edestruct IHpf as [st2' [exe' HQ]]; eauto.
+      inv_ceval. inv_ceval. eauto.
+    - inv_ceval. edestruct IHpf; eauto.
+      apply_sound. eauto.
+    - apply_sound.
+      edestruct H as [st' [exe' HQ]]; eauto.
+      edestruct IHpf as [st2' [? ?]]; eauto.
+  Qed.
 
-Ltac apply_sound :=
-  match goal with
-  | H : context[|- {{_}} _ {{_}}] |- _ =>
-    eapply hoare_proof_sound in H
-  | H : context[|- {[_]} _ {[_]}#] |- _ =>
-    eapply ehoare_proof_sound in H
-  end.
+  Definition rwp {env : Env} c (Q : Assertion2) : Assertion2 :=
+    fun st1 st2 => exists st2' (exe : st2 =[ c ]=> st2'), Q st1 st2'.
 
-Theorem rhle_proof_sound : forall P c1 c2 Q,
-    |- {{P}} c1 ~# c2 {[Q]} -> {{P}} c1 ~# c2 {[Q]}.
-Proof.
-  intros ? ? ? ? pf.
-  unfold rhle_triple.
-  induction pf; intros st1 st2 st1' exe HP.
-  - inv_ceval. eauto.
-  - firstorder eauto.
-  - edestruct IHpf as [st2' [exe' HQ]]; eauto.
-    inv_ceval. inv_ceval. eauto.
-  - inv_ceval. edestruct IHpf; eauto.
-    apply_sound. eauto.
-  - apply_sound.
-    edestruct H as [st' [exe' HQ]]; eauto.
-    edestruct IHpf as [st2' [? ?]]; eauto.
-Qed.
-
-Definition rwp c (Q : Assertion2) : Assertion2 :=
-  fun st1 st2 => exists st2' (exe : st2 =[ c ]=> st2'), Q st1 st2'.
-
-Theorem rhle_proof_complete : forall P c1 c2 Q,
-    {{P}} c1 ~# c2 {[Q]} -> |- {{P}} c1 ~# c2 {[Q]}.
-Proof.
-  unfold rhle_triple.
-  intros P c1 c2 Q H.
-  apply RHE_SkipIntroL. apply RHE_StepL with (rwp c2 Q).
-  intros st2. apply hoare_proof_complete.
-  firstorder.
-  apply RHE_SkipIntroR. eapply RHE_StepR. 2: constructor.
-  intros st1. apply ehoare_proof_complete.
-  firstorder.
-Qed.
+  Theorem rhle_proof_complete Sigma : forall P c1 c2 Q,
+      @rhle_triple {| funSpecs := Sigma; funDefs := empty |} P c1 c2 Q -> 
+      Sigma |- {{P}} c1 ~# c2 {[Q]}.
+  Proof.
+    unfold rhle_triple.
+    intros P c1 c2 Q H.
+    apply RHE_SkipIntroL. apply RHE_StepL with (@rwp {| funSpecs := Sigma; funDefs := empty |} c2 Q).
+    intros st2. apply hoare_proof_complete.
+    firstorder.
+    apply RHE_SkipIntroR. eapply RHE_StepR. 2: constructor.
+    intros st1. apply ehoare_proof_complete.
+    firstorder.
+  Qed.
 
 End RHLE.
 
@@ -107,6 +110,6 @@ Notation "{{ P }}  c1 ~# c2  {[ Q ]}" :=
   (rhle_triple P c1 c2 Q) (at level 90, c1 at next level, c2 at next level)
   : hoare_spec_scope.
 
-Notation "|- {{ P }}  c1 ~# c2  {[ Q ]}" :=
-  (rhle_proof P c1 c2 Q) (at level 90, c1 at next level, c2 at next level)
+Notation "Sigma |- {{ P }}  c1 ~# c2  {[ Q ]}" :=
+  (rhle_proof Sigma P c1 c2 Q) (at level 90, c1 at next level, c2 at next level)
   : hoare_spec_scope.
